impredicative_set/imonad_lib.v
@@ -26,6 +26,8 @@ Require Import ihierarchy.
 (*           algebraicity op == the operation op is algebraic                 *)
 (*          E .-aoperation M == algebraic E.-operation M                      *)
 (*         Monad_of_ret_bind == factory to build a monad from ret and bind    *)
+(*             commute m n f := (m >>= n >>= f) = (n >>= m >>= f)             *) 
+(*                              (ref: definition 4.2, mu2019tr3)              *)
 (*                                                                            *)
 (******************************************************************************)
 
@@ -55,8 +57,39 @@ bind_ext => ?; by rewrite bindretf /= -foldl_rev.
 Qed.
 Local Close Scope mprog.
 
-Definition liftM2 {M : monad} (A B C : UU0) (oplus : A -> B -> C) m1 m2 : M C :=
-  m1 >>= (fun x1 => m2 >>= (fun x2 => Ret (oplus x1 x2))).
+Definition liftM2 {M : monad} (A B C : UU0) (h : A -> B -> C) m1 m2 : M C :=
+  m1 >>= (fun a => m2 >>= (fun b => Ret (h a b))).
+
+Section liftM2_lemmas.
+Variables (M : monad) (A B C : UU0) (h : A -> B -> C).
+
+Lemma liftM2E m1 m2 D (f : C -> M D) : liftM2 h m1 m2 >>= f =
+  m1 >>= (fun x => m2 >>= fun y => f (h x y)) :> M _.
+Proof.
+rewrite /liftM2 bindA; under eq_bind do rewrite bindA.
+by bind_ext => s; under eq_bind do rewrite bindretf.
+Qed.
+
+Lemma liftM2_ret a b : liftM2 h (Ret a) (Ret b) = Ret (h a b) :> M _.
+Proof. by rewrite /liftM2 !bindretf. Qed.
+
+Lemma bind_liftM2_size (f : seq A -> seq B -> seq C)
+    (m1 : M (seq A)) (m2 : M (seq B)) n :
+  (forall a b, size (f a b) = size a + size b + n) ->
+  liftM2 f m1 m2 >>= (fun x => Ret (x, size x)) =
+  liftM2 (fun a b => (f a.1 b.1, a.2 + b.2 + n))
+          (m1 >>= (fun x => Ret (x, size x)))
+          (m2 >>= (fun x => Ret (x, size x))).
+Proof.
+move=> hf.
+rewrite /liftM2 !bindA; bind_ext => x1.
+rewrite !bindretf !bindA.
+bind_ext=> x2.
+by rewrite !bindretf /= hf.
+Qed.
+
+End liftM2_lemmas.
+Arguments bind_liftM2_size {M A B C} {f} m1 m2 n.
 
 Definition Squaring (A : UU0) := (A * A)%type.
 Notation "A `2" := (Squaring A).
@@ -504,6 +537,9 @@ rewrite compE mpairE compE bind_fmap; bind_ext => a2.
 rewrite fcompE fmap_bind 2!compE bind_fmap; bind_ext => a3.
 by rewrite fcompE -(compE (M # f^`2)) (natural ret) FIdf.
 Qed.
+
+Definition commute {M : monad} A B (m : M A) (n : M B) C (f : A -> B -> M C) : Prop :=
+  m >>= (fun x => n >>= (fun y => f x y)) = n >>= (fun y => m >>= (fun x => f x y)) :> M _.
 
 (*Local Notation "[ \o f , .. , g , h ]" := (f \o .. (g \o h) ..)
   (at level 0) (*, format "[ \o '['  f , '/' .. , '/' g , '/' h ']' ]"
